eIris/proofmode/reduction.v
@@ -1,0 +1,78 @@
+From elpi Require Import elpi.
+
+From iris.bi Require Import bi telescopes.
+From iris.proofmode Require Import base environments.
+From iris.prelude Require Import options.
+
+From eIris.proofmode.elpi Extra Dependency "reduction.elpi" as reduction.
+
+Elpi Db reduction.db lp:{{
+  pred reduction-rule o:constant.
+}}.
+
+Elpi Command EI.reduction.
+Elpi Accumulate Db reduction.db.
+Elpi Accumulate File reduction.
+Elpi Accumulate lp:{{
+
+  main [trm (global (const C))] :-
+    add-reduction-rule C.
+
+  main [trm (app [global (const C)| _ ])] :-
+    add-reduction-rule C.
+
+  main [] :-
+    all-reductions CS,
+    coq.say CS.
+  
+  main Args :-
+    coq.say "EI.reduction only accepts constants, not" Args.
+
+}}.
+Elpi Typecheck.
+Elpi Export EI.reduction.
+
+(* base *)
+EI.reduction (base.negb).
+EI.reduction (base.beq).
+EI.reduction (base.Pos_succ).
+EI.reduction (base.ascii_beq).
+EI.reduction (base.string_beq).
+EI.reduction (base.positive_beq).
+EI.reduction (base.ident_beq).
+
+(* environments *)
+EI.reduction (env_lookup).
+EI.reduction (env_lookup_delete).
+EI.reduction (env_delete).
+EI.reduction (env_app).
+EI.reduction (env_replace).
+EI.reduction (env_dom).
+EI.reduction (env_intuitionistic).
+EI.reduction (env_spatial).
+EI.reduction (env_counter).
+EI.reduction (env_spatial_is_nil).
+EI.reduction (envs_dom).
+EI.reduction (envs_lookup).
+EI.reduction (envs_lookup_delete).
+EI.reduction (envs_delete).
+EI.reduction (envs_snoc).
+EI.reduction (envs_app).
+EI.reduction (envs_simple_replace).
+EI.reduction (envs_replace).
+EI.reduction (envs_split).
+EI.reduction (envs_clear_spatial).
+EI.reduction (envs_clear_intuitionistic).
+EI.reduction (envs_incr_counter).
+EI.reduction (envs_split_go).
+EI.reduction (envs_split).
+EI.reduction (env_to_prop_go).
+EI.reduction (env_to_prop).
+EI.reduction (env_to_prop_and_go).
+EI.reduction (env_to_prop_and).
+
+(* PM list and option functions *)
+EI.reduction (pm_app).
+EI.reduction (pm_option_bind).
+EI.reduction (pm_from_option).
+EI.reduction (pm_option_fun).
